venom/props/stateEquivPropsScript.sml
@@ -1,0 +1,671 @@
+(*
+ * State Equivalence Properties (Statements Only)
+ *
+ * Re-exports all theorems from stateEquivProofs via ACCEPT_TAC.
+ * Proofs live in proofs/stateEquivProofsScript.sml.
+ *)
+
+Theory stateEquivProps
+Ancestors
+  stateEquivProofs
+
+(* ==========================================================================
+   Equivalence Relation Properties
+   ========================================================================== *)
+
+Theorem state_equiv_refl:
+  !s. state_equiv s s
+Proof
+  ACCEPT_TAC stateEquivProofsTheory.state_equiv_refl
+QED
+
+Theorem state_equiv_sym:
+  !s1 s2. state_equiv s1 s2 ==> state_equiv s2 s1
+Proof
+  ACCEPT_TAC stateEquivProofsTheory.state_equiv_sym
+QED
+
+Theorem state_equiv_trans:
+  !s1 s2 s3. state_equiv s1 s2 /\ state_equiv s2 s3 ==> state_equiv s1 s3
+Proof
+  ACCEPT_TAC stateEquivProofsTheory.state_equiv_trans
+QED
+
+(* ==========================================================================
+   Result Equivalence Properties
+   ========================================================================== *)
+
+Theorem result_equiv_refl:
+  !r. result_equiv r r
+Proof
+  ACCEPT_TAC stateEquivProofsTheory.result_equiv_refl
+QED
+
+Theorem result_equiv_error[simp]:
+  result_equiv (Error e) (Error e) = T
+Proof
+  ACCEPT_TAC stateEquivProofsTheory.result_equiv_error
+QED
+
+Theorem result_equiv_ok[simp]:
+  result_equiv (OK s1) (OK s2) = state_equiv s1 s2
+Proof
+  ACCEPT_TAC stateEquivProofsTheory.result_equiv_ok
+QED
+
+Theorem result_equiv_halt[simp]:
+  result_equiv (Halt s1) (Halt s2) = state_equiv s1 s2
+Proof
+  ACCEPT_TAC stateEquivProofsTheory.result_equiv_halt
+QED
+
+Theorem result_equiv_revert[simp]:
+  result_equiv (Revert s1) (Revert s2) = state_equiv s1 s2
+Proof
+  ACCEPT_TAC stateEquivProofsTheory.result_equiv_revert
+QED
+
+Theorem result_equiv_error_any[simp]:
+  result_equiv (Error e1) (Error e2) = T
+Proof
+  ACCEPT_TAC stateEquivProofsTheory.result_equiv_error_any
+QED
+
+Theorem result_equiv_mismatch[simp]:
+  result_equiv (OK s) (Halt s') = F /\
+  result_equiv (OK s) (Revert s') = F /\
+  result_equiv (OK s) (Error e) = F /\
+  result_equiv (Halt s) (OK s') = F /\
+  result_equiv (Halt s) (Revert s') = F /\
+  result_equiv (Halt s) (Error e) = F /\
+  result_equiv (Revert s) (OK s') = F /\
+  result_equiv (Revert s) (Halt s') = F /\
+  result_equiv (Revert s) (Error e) = F /\
+  result_equiv (Error e) (OK s) = F /\
+  result_equiv (Error e) (Halt s) = F /\
+  result_equiv (Error e) (Revert s) = F
+Proof
+  ACCEPT_TAC stateEquivProofsTheory.result_equiv_mismatch
+QED
+
+(* ==========================================================================
+   Operand Evaluation Preserves Equivalence
+   ========================================================================== *)
+
+Theorem eval_operand_state_equiv:
+  !op s1 s2.
+    state_equiv s1 s2 ==>
+    eval_operand op s1 = eval_operand op s2
+Proof
+  ACCEPT_TAC stateEquivProofsTheory.eval_operand_state_equiv
+QED
+
+(* ==========================================================================
+   State Mutation Operations Preserve Equivalence
+   ========================================================================== *)
+
+Theorem update_var_state_equiv:
+  !x v s1 s2.
+    state_equiv s1 s2 ==>
+    state_equiv (update_var x v s1) (update_var x v s2)
+Proof
+  ACCEPT_TAC stateEquivProofsTheory.update_var_state_equiv
+QED
+
+Theorem mload_state_equiv:
+  !offset s1 s2.
+    state_equiv s1 s2 ==>
+    mload offset s1 = mload offset s2
+Proof
+  ACCEPT_TAC stateEquivProofsTheory.mload_state_equiv
+QED
+
+Theorem mstore_state_equiv:
+  !offset v s1 s2.
+    state_equiv s1 s2 ==>
+    state_equiv (mstore offset v s1) (mstore offset v s2)
+Proof
+  ACCEPT_TAC stateEquivProofsTheory.mstore_state_equiv
+QED
+
+Theorem write_memory_with_expansion_state_equiv:
+  !offset bytes s1 s2.
+    state_equiv s1 s2 ==>
+    state_equiv (write_memory_with_expansion offset bytes s1)
+                (write_memory_with_expansion offset bytes s2)
+Proof
+  ACCEPT_TAC stateEquivProofsTheory.write_memory_with_expansion_state_equiv
+QED
+
+Theorem sload_state_equiv:
+  !key s1 s2.
+    state_equiv s1 s2 ==>
+    sload key s1 = sload key s2
+Proof
+  ACCEPT_TAC stateEquivProofsTheory.sload_state_equiv
+QED
+
+Theorem sstore_state_equiv:
+  !key v s1 s2.
+    state_equiv s1 s2 ==>
+    state_equiv (sstore key v s1) (sstore key v s2)
+Proof
+  ACCEPT_TAC stateEquivProofsTheory.sstore_state_equiv
+QED
+
+Theorem tload_state_equiv:
+  !key s1 s2.
+    state_equiv s1 s2 ==>
+    tload key s1 = tload key s2
+Proof
+  ACCEPT_TAC stateEquivProofsTheory.tload_state_equiv
+QED
+
+Theorem tstore_state_equiv:
+  !key v s1 s2.
+    state_equiv s1 s2 ==>
+    state_equiv (tstore key v s1) (tstore key v s2)
+Proof
+  ACCEPT_TAC stateEquivProofsTheory.tstore_state_equiv
+QED
+
+Theorem jump_to_state_equiv:
+  !lbl s1 s2.
+    state_equiv s1 s2 ==>
+    state_equiv (jump_to lbl s1) (jump_to lbl s2)
+Proof
+  ACCEPT_TAC stateEquivProofsTheory.jump_to_state_equiv
+QED
+
+Theorem halt_state_state_equiv:
+  !s1 s2.
+    state_equiv s1 s2 ==>
+    state_equiv (halt_state s1) (halt_state s2)
+Proof
+  ACCEPT_TAC stateEquivProofsTheory.halt_state_state_equiv
+QED
+
+Theorem revert_state_state_equiv:
+  !s1 s2.
+    state_equiv s1 s2 ==>
+    state_equiv (revert_state s1) (revert_state s2)
+Proof
+  ACCEPT_TAC stateEquivProofsTheory.revert_state_state_equiv
+QED
+
+(* ==========================================================================
+   Equivalence Relation Properties for observable_equiv
+   ========================================================================== *)
+
+Theorem observable_equiv_refl:
+  !s. observable_equiv s s
+Proof
+  ACCEPT_TAC stateEquivProofsTheory.observable_equiv_refl
+QED
+
+Theorem observable_equiv_sym:
+  !s1 s2. observable_equiv s1 s2 ==> observable_equiv s2 s1
+Proof
+  ACCEPT_TAC stateEquivProofsTheory.observable_equiv_sym
+QED
+
+Theorem observable_equiv_trans:
+  !s1 s2 s3.
+    observable_equiv s1 s2 /\ observable_equiv s2 s3 ==>
+    observable_equiv s1 s3
+Proof
+  ACCEPT_TAC stateEquivProofsTheory.observable_equiv_trans
+QED
+
+(* ==========================================================================
+   Equivalence Relation Properties for execution_equiv_except
+   ========================================================================== *)
+
+Theorem execution_equiv_except_refl:
+  !vars s. execution_equiv_except vars s s
+Proof
+  ACCEPT_TAC stateEquivProofsTheory.execution_equiv_except_refl
+QED
+
+Theorem execution_equiv_except_sym:
+  !vars s1 s2.
+    execution_equiv_except vars s1 s2 ==>
+    execution_equiv_except vars s2 s1
+Proof
+  ACCEPT_TAC stateEquivProofsTheory.execution_equiv_except_sym
+QED
+
+Theorem execution_equiv_except_trans:
+  !vars s1 s2 s3.
+    execution_equiv_except vars s1 s2 /\
+    execution_equiv_except vars s2 s3 ==>
+    execution_equiv_except vars s1 s3
+Proof
+  ACCEPT_TAC stateEquivProofsTheory.execution_equiv_except_trans
+QED
+
+Theorem execution_equiv_except_subset:
+  !vars1 vars2 s1 s2.
+    execution_equiv_except vars1 s1 s2 /\
+    vars1 SUBSET vars2 ==>
+    execution_equiv_except vars2 s1 s2
+Proof
+  ACCEPT_TAC stateEquivProofsTheory.execution_equiv_except_subset
+QED
+
+(* ==========================================================================
+   Equivalence Relation Properties for state_equiv_except
+   ========================================================================== *)
+
+Theorem state_equiv_except_refl:
+  !vars s. state_equiv_except vars s s
+Proof
+  ACCEPT_TAC stateEquivProofsTheory.state_equiv_except_refl
+QED
+
+Theorem state_equiv_except_sym:
+  !vars s1 s2.
+    state_equiv_except vars s1 s2 ==>
+    state_equiv_except vars s2 s1
+Proof
+  ACCEPT_TAC stateEquivProofsTheory.state_equiv_except_sym
+QED
+
+Theorem state_equiv_except_trans:
+  !vars s1 s2 s3.
+    state_equiv_except vars s1 s2 /\
+    state_equiv_except vars s2 s3 ==>
+    state_equiv_except vars s1 s3
+Proof
+  ACCEPT_TAC stateEquivProofsTheory.state_equiv_except_trans
+QED
+
+Theorem state_equiv_implies_except:
+  !vars s1 s2.
+    state_equiv s1 s2 ==>
+    state_equiv_except vars s1 s2
+Proof
+  ACCEPT_TAC stateEquivProofsTheory.state_equiv_implies_except
+QED
+
+Theorem state_equiv_except_empty:
+  !s1 s2.
+    state_equiv_except {} s1 s2 <=>
+    (!v. lookup_var v s1 = lookup_var v s2) /\
+    s1.vs_memory = s2.vs_memory /\
+    s1.vs_storage = s2.vs_storage /\
+    s1.vs_transient = s2.vs_transient /\
+    s1.vs_current_bb = s2.vs_current_bb /\
+    s1.vs_inst_idx = s2.vs_inst_idx /\
+    s1.vs_prev_bb = s2.vs_prev_bb /\
+    s1.vs_halted = s2.vs_halted /\
+    s1.vs_reverted = s2.vs_reverted /\
+    s1.vs_returndata = s2.vs_returndata /\
+    s1.vs_accounts = s2.vs_accounts /\
+    s1.vs_call_ctx = s2.vs_call_ctx /\
+    s1.vs_tx_ctx = s2.vs_tx_ctx /\
+    s1.vs_block_ctx = s2.vs_block_ctx
+Proof
+  ACCEPT_TAC stateEquivProofsTheory.state_equiv_except_empty
+QED
+
+(* ==========================================================================
+   Lifting Lemmas: Stronger Equivalence Implies Weaker
+   ========================================================================== *)
+
+Theorem state_equiv_except_implies_execution:
+  !vars s1 s2.
+    state_equiv_except vars s1 s2 ==>
+    execution_equiv_except vars s1 s2
+Proof
+  ACCEPT_TAC stateEquivProofsTheory.state_equiv_except_implies_execution
+QED
+
+Theorem execution_equiv_except_implies_observable:
+  !vars s1 s2.
+    execution_equiv_except vars s1 s2 ==>
+    observable_equiv s1 s2
+Proof
+  ACCEPT_TAC stateEquivProofsTheory.execution_equiv_except_implies_observable
+QED
+
+Theorem state_equiv_except_implies_observable:
+  !vars s1 s2.
+    state_equiv_except vars s1 s2 ==>
+    observable_equiv s1 s2
+Proof
+  ACCEPT_TAC stateEquivProofsTheory.state_equiv_except_implies_observable
+QED
+
+(* ==========================================================================
+   Result Equivalence with Variable Exceptions - Properties
+   ========================================================================== *)
+
+Theorem result_equiv_except_refl:
+  !vars r. result_equiv_except vars r r
+Proof
+  ACCEPT_TAC stateEquivProofsTheory.result_equiv_except_refl
+QED
+
+Theorem result_equiv_except_ok[simp]:
+  result_equiv_except vars (OK s1) (OK s2) = state_equiv_except vars s1 s2
+Proof
+  ACCEPT_TAC stateEquivProofsTheory.result_equiv_except_ok
+QED
+
+Theorem result_equiv_except_halt[simp]:
+  result_equiv_except vars (Halt s1) (Halt s2) = execution_equiv_except vars s1 s2
+Proof
+  ACCEPT_TAC stateEquivProofsTheory.result_equiv_except_halt
+QED
+
+Theorem result_equiv_except_revert[simp]:
+  result_equiv_except vars (Revert s1) (Revert s2) = execution_equiv_except vars s1 s2
+Proof
+  ACCEPT_TAC stateEquivProofsTheory.result_equiv_except_revert
+QED
+
+Theorem result_equiv_except_error[simp]:
+  result_equiv_except vars (Error e1) (Error e2) = T
+Proof
+  ACCEPT_TAC stateEquivProofsTheory.result_equiv_except_error
+QED
+
+Theorem result_equiv_except_mismatch[simp]:
+  result_equiv_except vars (OK s) (Halt s') = F /\
+  result_equiv_except vars (OK s) (Revert s') = F /\
+  result_equiv_except vars (OK s) (Error e) = F /\
+  result_equiv_except vars (Halt s) (OK s') = F /\
+  result_equiv_except vars (Halt s) (Revert s') = F /\
+  result_equiv_except vars (Halt s) (Error e) = F /\
+  result_equiv_except vars (Revert s) (OK s') = F /\
+  result_equiv_except vars (Revert s) (Halt s') = F /\
+  result_equiv_except vars (Revert s) (Error e) = F /\
+  result_equiv_except vars (Error e) (OK s) = F /\
+  result_equiv_except vars (Error e) (Halt s) = F /\
+  result_equiv_except vars (Error e) (Revert s) = F
+Proof
+  ACCEPT_TAC stateEquivProofsTheory.result_equiv_except_mismatch
+QED
+
+(* ==========================================================================
+   Update Preserves execution_equiv_except
+   ========================================================================== *)
+
+Theorem update_var_in_execution_equiv_preserves:
+  !vars x v1 v2 s1 s2.
+    x IN vars /\
+    execution_equiv_except vars s1 s2 ==>
+    execution_equiv_except vars (update_var x v1 s1) (update_var x v2 s2)
+Proof
+  ACCEPT_TAC stateEquivProofsTheory.update_var_in_execution_equiv_preserves
+QED
+
+Theorem update_var_same_execution_equiv_preserves:
+  !vars x v s1 s2.
+    execution_equiv_except vars s1 s2 ==>
+    execution_equiv_except vars (update_var x v s1) (update_var x v s2)
+Proof
+  ACCEPT_TAC stateEquivProofsTheory.update_var_same_execution_equiv_preserves
+QED
+
+Theorem update_var_execution_equiv_one_side:
+  !vars x v s1 s2.
+    x IN vars /\
+    execution_equiv_except vars s1 s2 ==>
+    execution_equiv_except vars (update_var x v s1) s2
+Proof
+  ACCEPT_TAC stateEquivProofsTheory.update_var_execution_equiv_one_side
+QED
+
+(* ==========================================================================
+   Update Preserves state_equiv_except
+   ========================================================================== *)
+
+Theorem update_var_in_except_preserves:
+  !vars x v1 v2 s1 s2.
+    x IN vars /\
+    state_equiv_except vars s1 s2 ==>
+    state_equiv_except vars (update_var x v1 s1) (update_var x v2 s2)
+Proof
+  ACCEPT_TAC stateEquivProofsTheory.update_var_in_except_preserves
+QED
+
+Theorem update_var_same_preserves:
+  !vars x v s1 s2.
+    state_equiv_except vars s1 s2 ==>
+    state_equiv_except vars (update_var x v s1) (update_var x v s2)
+Proof
+  ACCEPT_TAC stateEquivProofsTheory.update_var_same_preserves
+QED
+
+Theorem update_var_except_one_side:
+  !vars x v s1 s2.
+    x IN vars /\
+    state_equiv_except vars s1 s2 ==>
+    state_equiv_except vars (update_var x v s1) s2
+Proof
+  ACCEPT_TAC stateEquivProofsTheory.update_var_except_one_side
+QED
+
+(* ==========================================================================
+   Operand Evaluation under equivalence
+   ========================================================================== *)
+
+Theorem eval_operand_execution_equiv:
+  !vars op s1 s2.
+    execution_equiv_except vars s1 s2 /\
+    (!x. op = Var x ==> x NOTIN vars) ==>
+    eval_operand op s1 = eval_operand op s2
+Proof
+  ACCEPT_TAC stateEquivProofsTheory.eval_operand_execution_equiv
+QED
+
+Theorem eval_operand_except:
+  !vars op s1 s2.
+    state_equiv_except vars s1 s2 /\
+    (!x. op = Var x ==> x NOTIN vars) ==>
+    eval_operand op s1 = eval_operand op s2
+Proof
+  ACCEPT_TAC stateEquivProofsTheory.eval_operand_except
+QED
+
+(* ==========================================================================
+   Control Flow Preserves execution_equiv_except
+   ========================================================================== *)
+
+Theorem halt_state_execution_equiv_preserves:
+  !vars s1 s2.
+    execution_equiv_except vars s1 s2 ==>
+    execution_equiv_except vars (halt_state s1) (halt_state s2)
+Proof
+  ACCEPT_TAC stateEquivProofsTheory.halt_state_execution_equiv_preserves
+QED
+
+Theorem revert_state_execution_equiv_preserves:
+  !vars s1 s2.
+    execution_equiv_except vars s1 s2 ==>
+    execution_equiv_except vars (revert_state s1) (revert_state s2)
+Proof
+  ACCEPT_TAC stateEquivProofsTheory.revert_state_execution_equiv_preserves
+QED
+
+Theorem halt_state_from_state_except:
+  !vars s1 s2.
+    state_equiv_except vars s1 s2 ==>
+    execution_equiv_except vars (halt_state s1) (halt_state s2)
+Proof
+  ACCEPT_TAC stateEquivProofsTheory.halt_state_from_state_except
+QED
+
+Theorem revert_state_from_state_except:
+  !vars s1 s2.
+    state_equiv_except vars s1 s2 ==>
+    execution_equiv_except vars (revert_state s1) (revert_state s2)
+Proof
+  ACCEPT_TAC stateEquivProofsTheory.revert_state_from_state_except
+QED
+
+(* ==========================================================================
+   Control Flow Preserves state_equiv_except
+   ========================================================================== *)
+
+Theorem jump_to_except_preserves:
+  !vars lbl s1 s2.
+    state_equiv_except vars s1 s2 ==>
+    state_equiv_except vars (jump_to lbl s1) (jump_to lbl s2)
+Proof
+  ACCEPT_TAC stateEquivProofsTheory.jump_to_except_preserves
+QED
+
+Theorem halt_state_except_preserves:
+  !vars s1 s2.
+    state_equiv_except vars s1 s2 ==>
+    state_equiv_except vars (halt_state s1) (halt_state s2)
+Proof
+  ACCEPT_TAC stateEquivProofsTheory.halt_state_except_preserves
+QED
+
+Theorem revert_state_except_preserves:
+  !vars s1 s2.
+    state_equiv_except vars s1 s2 ==>
+    state_equiv_except vars (revert_state s1) (revert_state s2)
+Proof
+  ACCEPT_TAC stateEquivProofsTheory.revert_state_except_preserves
+QED
+
+(* ==========================================================================
+   Widening the Exception Set
+   ========================================================================== *)
+
+Theorem state_equiv_except_subset:
+  !vars1 vars2 s1 s2.
+    state_equiv_except vars1 s1 s2 /\
+    vars1 SUBSET vars2 ==>
+    state_equiv_except vars2 s1 s2
+Proof
+  ACCEPT_TAC stateEquivProofsTheory.state_equiv_except_subset
+QED
+
+Theorem result_equiv_except_subset:
+  !vars1 vars2 r1 r2.
+    result_equiv_except vars1 r1 r2 /\
+    vars1 SUBSET vars2 ==>
+    result_equiv_except vars2 r1 r2
+Proof
+  ACCEPT_TAC stateEquivProofsTheory.result_equiv_except_subset
+QED
+
+(* ==========================================================================
+   Memory/Storage Operations Preserve execution_equiv_except
+   ========================================================================== *)
+
+Theorem mstore_execution_equiv_preserves:
+  !vars addr val s1 s2.
+    execution_equiv_except vars s1 s2 ==>
+    execution_equiv_except vars (mstore addr val s1) (mstore addr val s2)
+Proof
+  ACCEPT_TAC stateEquivProofsTheory.mstore_execution_equiv_preserves
+QED
+
+Theorem mload_execution_equiv_same:
+  !vars addr s1 s2.
+    execution_equiv_except vars s1 s2 ==>
+    mload addr s1 = mload addr s2
+Proof
+  ACCEPT_TAC stateEquivProofsTheory.mload_execution_equiv_same
+QED
+
+Theorem sstore_execution_equiv_preserves:
+  !vars key val s1 s2.
+    execution_equiv_except vars s1 s2 ==>
+    execution_equiv_except vars (sstore key val s1) (sstore key val s2)
+Proof
+  ACCEPT_TAC stateEquivProofsTheory.sstore_execution_equiv_preserves
+QED
+
+Theorem sload_execution_equiv_same:
+  !vars key s1 s2.
+    execution_equiv_except vars s1 s2 ==>
+    sload key s1 = sload key s2
+Proof
+  ACCEPT_TAC stateEquivProofsTheory.sload_execution_equiv_same
+QED
+
+Theorem tstore_execution_equiv_preserves:
+  !vars key val s1 s2.
+    execution_equiv_except vars s1 s2 ==>
+    execution_equiv_except vars (tstore key val s1) (tstore key val s2)
+Proof
+  ACCEPT_TAC stateEquivProofsTheory.tstore_execution_equiv_preserves
+QED
+
+Theorem tload_execution_equiv_same:
+  !vars key s1 s2.
+    execution_equiv_except vars s1 s2 ==>
+    tload key s1 = tload key s2
+Proof
+  ACCEPT_TAC stateEquivProofsTheory.tload_execution_equiv_same
+QED
+
+(* ==========================================================================
+   Memory/Storage Operations Preserve state_equiv_except
+   ========================================================================== *)
+
+Theorem mstore_except_preserves:
+  !vars addr val s1 s2.
+    state_equiv_except vars s1 s2 ==>
+    state_equiv_except vars (mstore addr val s1) (mstore addr val s2)
+Proof
+  ACCEPT_TAC stateEquivProofsTheory.mstore_except_preserves
+QED
+
+Theorem mload_except_same:
+  !vars addr s1 s2.
+    state_equiv_except vars s1 s2 ==>
+    mload addr s1 = mload addr s2
+Proof
+  ACCEPT_TAC stateEquivProofsTheory.mload_except_same
+QED
+
+Theorem sstore_except_preserves:
+  !vars key val s1 s2.
+    state_equiv_except vars s1 s2 ==>
+    state_equiv_except vars (sstore key val s1) (sstore key val s2)
+Proof
+  ACCEPT_TAC stateEquivProofsTheory.sstore_except_preserves
+QED
+
+Theorem sload_except_same:
+  !vars key s1 s2.
+    state_equiv_except vars s1 s2 ==>
+    sload key s1 = sload key s2
+Proof
+  ACCEPT_TAC stateEquivProofsTheory.sload_except_same
+QED
+
+Theorem tstore_except_preserves:
+  !vars key val s1 s2.
+    state_equiv_except vars s1 s2 ==>
+    state_equiv_except vars (tstore key val s1) (tstore key val s2)
+Proof
+  ACCEPT_TAC stateEquivProofsTheory.tstore_except_preserves
+QED
+
+Theorem tload_except_same:
+  !vars key s1 s2.
+    state_equiv_except vars s1 s2 ==>
+    tload key s1 = tload key s2
+Proof
+  ACCEPT_TAC stateEquivProofsTheory.tload_except_same
+QED
+
+Theorem write_memory_with_expansion_except_preserves:
+  !vars offset bytes s1 s2.
+    state_equiv_except vars s1 s2 ==>
+    state_equiv_except vars
+      (write_memory_with_expansion offset bytes s1)
+      (write_memory_with_expansion offset bytes s2)
+Proof
+  ACCEPT_TAC stateEquivProofsTheory.write_memory_with_expansion_except_preserves
+QED
